More normalization rules

Refinement.v
@@ -5,7 +5,7 @@ Ltac inv H := inversion H; clear H; subst;
               repeat match goal with
                      | [ H : existT _ _ _ = existT _ _ _ |- _ ] =>
                        apply (inj_pair2_eq_dec _ string_dec) in H; subst
-                     end.
+                     end; simpl in *.
 
 Section Refinement.
   Variable chs : channels.
@@ -44,6 +44,108 @@ Section Refinement.
     refines p (procsD ps)
     /\ refines (procsD ps) p.
 
+  CoInductive normalize : process chs -> proc0 -> Prop :=
+  | InSend : forall ch v k k', normalize k k'
+    -> normalize (DoSend ch v k) (NSend ch v k')
+  | InRecv : forall ch k k', (forall v, normalize (k v) (k' v))
+    -> normalize (DoRecv ch k) (NRecv ch k')
+  | InDone : normalize Done NDone.
+
+  Lemma expand_proc0D : forall p, proc0D p = expand (proc0D p).
+  Proof.
+    intros.
+    rewrite <- expand_ok.
+    auto.
+  Qed.
+
+  Lemma normalize_fwd : forall p tr, traceOf p tr
+    -> forall p', normalize p p'
+      -> traceOf (proc0D p') tr.
+  Proof.
+    induction 1; simpl; eauto; inversion 1; subst.
+    apply (inj_pair2_eq_dec _ string_dec) in H3; subst.
+    rewrite expand_proc0D in *; simpl in *.
+    eauto.
+    apply (inj_pair2_eq_dec _ string_dec) in H3; subst.
+    rewrite expand_proc0D in *; simpl in *.
+    eauto.
+  Qed.
+
+
+  Lemma normalize_bwd : forall p'0 tr, traceOf p'0 tr
+    -> forall p p', normalize p p'
+      -> p'0 = proc0D p'
+      -> traceOf p tr.
+  Proof.
+    induction 1; simpl; eauto; destruct 1; simpl; intros;
+    try match goal with
+        | [ H : _ = proc0D _ |- _ ] => rewrite expand_proc0D in H; simpl in H; inv H; eauto
+        end.
+
+    rewrite expand_proc0D in *; simpl in *.
+    inversion H1; clear H1.
+    destruct H3.
+    apply (inj_pair2_eq_dec _ string_dec) in H4; subst.
+    eauto.
+  Qed.
+
+  Lemma traceAll_True : forall p, traceAll (chs := chs) (fun _ => True) p.
+  Proof.
+    induction p; auto.
+  Qed.
+
+  Hint Resolve traceAll_True.
+
+  Lemma interleave_nil1' : forall nl tr1 tr2,
+    interleave (chs := chs) nl tr1 tr2
+    -> nl = nil
+    -> tr1 = tr2.
+  Proof.
+    induction 1; simpl; intros; intuition; try congruence.
+  Qed.
+
+  Lemma interleave_nil1 : forall tr1 tr2,
+    interleave (chs := chs) nil tr1 tr2
+    -> tr1 = tr2.
+  Proof.
+    eauto using interleave_nil1'.
+  Qed.
+
+  Lemma interleave_sym : forall tr1 tr2 tr3,
+    interleave (chs := chs) tr1 tr2 tr3
+    -> interleave tr2 tr1 tr3.
+  Proof.
+    induction 1; eauto.
+  Qed.
+
+  Lemma interleave_nil2 : forall tr1 tr2,
+    interleave (chs := chs) tr1 nil tr2
+    -> tr1 = tr2.
+  Proof.
+    intros; apply interleave_nil1; apply interleave_sym; auto.
+  Qed.
+
+  Theorem normBasic : forall p p', normalize p p'
+    -> norm p ({| Chans := fun _ => True; Code := p' |} :: nil).
+  Proof.
+    split; unfold procsD, procD; simpl.
+
+    do 2 intro.
+    econstructor.
+    2: eauto.
+    2: eauto.
+    econstructor.
+    eauto using normalize_fwd.
+    auto.
+
+    do 2 intro.
+    inv H0; eauto.
+    inv H4.
+    apply interleave_nil2 in H6; subst.
+    inv H3; eauto.
+    eauto using normalize_bwd.
+  Qed.
+
   Theorem normDone : norm Done ({| Chans := fun _ => True; Code := NDone |} :: nil).
   Proof.
     split; simpl; do 2 intro.
@@ -57,13 +159,6 @@ Section Refinement.
     inv H1; eauto.
     inv H5; eauto.
     inv H5; eauto.
-  Qed.
-
-  Lemma interleave_sym : forall tr1 tr2 tr3,
-    interleave (chs := chs) tr1 tr2 tr3
-    -> interleave tr2 tr1 tr3.
-  Proof.
-    induction 1; eauto.
   Qed.
 
   Theorem Parallel_comm : forall p1 p2,
@@ -137,21 +232,6 @@ Section Refinement.
     inv H; eauto.
   Qed.
 
-  Lemma interleave_nil1' : forall nl tr1 tr2,
-    interleave (chs := chs) nl tr1 tr2
-    -> nl = nil
-    -> tr1 = tr2.
-  Proof.
-    induction 1; simpl; intros; intuition; try congruence.
-  Qed.
-
-  Lemma interleave_nil1 : forall tr1 tr2,
-    interleave (chs := chs) nil tr1 tr2
-    -> tr1 = tr2.
-  Proof.
-    eauto using interleave_nil1'.
-  Qed.
-
   Lemma procsD_app2 : forall ps2 ps1,
     refines (Parallel (procsD ps1) (procsD ps2)) (procsD (ps1 ++ ps2)%list).
   Proof.
@@ -182,53 +262,90 @@ Section Refinement.
     inv H1; eauto.
   Qed.
 
-  Theorem normSend : forall ch v k p,
-    norm k (p :: nil)
-    -> Chans p (Send, ch)
-    -> norm (DoSend ch v k) ({| Chans := Chans p; Code := NSend ch v (Code p) |} :: nil).
+  Lemma traceAll_and : forall P1 P2 tr,
+    traceAll (chs := chs) P1 tr
+    -> traceAll P2 tr
+    -> traceAll (fun x => P1 x /\ P2 x) tr.
   Proof.
-    unfold norm, refines; simpl; intuition.
+    induction 1; inversion 1; subst; eauto.
+    constructor; intuition.
+  Qed.
+
+  Lemma traceAll_weaken : forall (P1 P2 : _ -> Prop),
+    (forall x, P1 x -> P2 x)
+    -> forall ps, traceAll (chs := chs) P1 ps
+      -> traceAll P2 ps.
+  Proof.
+    induction 2; eauto.
+  Qed.
+
+  Theorem normRestrict1 : forall (P : _ -> Prop) p p',
+    norm p (p' :: nil)
+    -> norm (Restrict P p) ({| Code := Code p';
+                               Chans := fun x => P x /\ Chans p' x |} :: nil).
+  Proof.
+    unfold norm, refines, procsD, procD; simpl; intuition.
 
     inv H; eauto.
-    apply H1 in H7; clear H1.
-    inv H7; eauto.
-    inv H4.
-    apply interleave_sym in H6; apply interleave_nil1 in H6; subst.
-    unfold procD in *; simpl in *.
-    inv H3; eauto.
+    apply H0 in H4; clear H0.
+    inv H4; eauto.
+    inv H3.
+    apply interleave_nil2 in H7; subst.
+    inv H2; eauto.
     econstructor.
     2: eauto.
     2: eauto.
     econstructor.
-    rewrite (expand_ok (proc0D (NSend ch v (Code p)))); simpl.
     eauto.
-    eauto.
-    econstructor.
-    2: eauto.
-    2: eauto.
-    econstructor.
-    rewrite (expand_ok (proc0D (NSend ch v (Code p)))); simpl.
-    eauto.
-    eauto.
-    econstructor.
-    2: eauto.
-    2: eauto.
-    econstructor.
-    simpl.
-    rewrite (expand_ok (proc0D (NSend ch v (Code p)))); simpl.
-    eauto.
-    eauto.
+    auto using traceAll_and.
 
-    unfold procD in *; simpl in *.
     inv H; eauto.
-    inv H6.
-    apply interleave_sym in H8; apply interleave_nil1 in H8; subst.
-    inv H5; eauto.
-    rewrite (expand_ok (proc0D (NSend ch v (Code p)))) in *.
-    simpl in *.
+    inv H5.
+    apply interleave_nil2 in H7; subst.
     inv H4; eauto.
     econstructor; eauto.
-    apply H2.
-    inv H7; eauto.
+    apply H1.
+    econstructor.
+    2: eauto.
+    2: eauto.
+    2: eapply traceAll_weaken; [ | eassumption ]; cbv beta; tauto.
+    econstructor.
+    eauto.
+    eapply traceAll_weaken; [ | eassumption ]; cbv beta; tauto.
   Qed.
+
+  Lemma traceAll_interleave : forall tr1 tr2 tr, interleave (chs := chs) tr1 tr2 tr
+    -> forall P, traceAll P tr1
+      -> traceAll P tr2
+      -> traceAll P tr.
+  Proof.
+    induction 1; inversion 1; subst; inversion 1; subst; eauto;
+    econstructor; eauto; apply IHinterleave; eauto.
+  Qed.
+
+  Theorem normRestrictMany : forall (P : _ -> Prop) p ps,
+    norm p ps
+    -> Forall (fun r => forall x, Chans r x -> P x) ps
+    -> norm (Restrict P p) ps.
+  Proof.
+    unfold norm, refines; intuition.
+
+    inv H; eauto.
+
+    econstructor.
+    auto.
+    clear H1 H2.
+    generalize dependent tr.
+    induction H0; simpl; intros.
+    inv H; eauto.
+    inv H1; eauto.
+    unfold procD in H4.
+    inv H4; eauto.
+    eapply traceAll_interleave; eauto.
+    eapply traceAll_weaken; eauto.
+
+    apply interleave_nil1 in H7; subst.
+    eauto.
+  Qed.    
+
 End Refinement.
